TM/Compound/Peek.v
@@ -1,0 +1,134 @@
+Require Import TM.Prelim TM.TM.
+Require Import TM.Basic.Mono.
+Require Import TM.Combinators.Match TM.Combinators.SequentialComposition.
+
+
+Section Peek.
+
+  Variable sig : finType.
+  Variable F : finType.
+  Variable f : sig -> F.
+
+  Definition peek_state := FinType (EqType (option (F + move))) % type.
+  Definition peek_start : peek_state := None.
+  Definition peek_Some (y : F) : peek_state := Some (inl y).
+  Definition peek_None (d : move) : peek_state := Some (inr d).
+
+
+  Definition Peek : { M : mTM sig 1 & states M -> F + move } :=
+    MATCH (Read_char _)
+          (fun r1 =>
+             match r1 with
+             | Some r1' => mono_Nop sig (inl (f r1'))
+             | None =>
+               Move sig L tt ;;
+                    MATCH (Read_char _)
+                    (fun r2 =>
+                       match r2 with
+                       | Some r2' => Move sig R (inr R)
+                       | None =>
+                         Move sig R tt ;;
+                              MATCH (Read_char _)
+                              (fun r3 =>
+                                 match r3 with
+                                 | Some r3' => Move sig L (inr L)
+                                 | None => mono_Nop sig (inr N)
+                                 end)
+                       end)
+             end).
+
+  Definition Peek_Rel : Rel (tapes sig 1) (FinType(EqType(F + move)) * tapes sig 1) :=
+    Mk_R_p (fun tin '(y, tout) => tin = tout /\
+                               match tin with
+                               | niltape _ => y = inr N
+                               | leftof _ _ => y = inr L
+                               | rightof _ _ => y = inr R
+                               | midtape _ m _ => y = inl (f m)
+                               end).
+
+  Definition Peek_Steps := 11.
+
+  Lemma Peek_RealisesIn :
+    Peek ⊨c(Peek_Steps) Peek_Rel.
+  Proof.
+    unfold Peek_Steps. eapply RealiseIn_monotone.
+    - unfold Peek. eapply Match_RealiseIn.
+      {
+        eapply read_char_sem.
+      }
+      {
+        intros r1. cbn in r1. instantiate (2 := fun (b : option sig) => match b with Some r1' => _ | None => _ end).
+        destruct r1 as [ r1' | ].
+        {
+          eapply RealiseIn_monotone. eapply mono_Nop_Sem. omega. intros x y H. apply H.
+        }
+        {
+          eapply Seq_RealiseIn.
+          {
+            eapply Move_Sem.
+          }
+          {
+            eapply Match_RealiseIn.
+            {
+              eapply read_char_sem.
+            }
+            {
+              intros r2. cbn in r2. instantiate (2 := fun (b : option sig) => match b with Some r2' => _ | None => _ end).
+              destruct r2 as [ r2' | ].
+              {
+                eapply RealiseIn_monotone. eapply Move_Sem. shelve. intros x y H. apply H.
+              }
+              {
+                eapply Seq_RealiseIn.
+                {
+                  eapply Move_Sem.
+                }
+                {
+                  eapply Match_RealiseIn.
+                  {
+                    eapply read_char_sem.
+                  }
+                  {
+                    intros r3. cbn in r3. instantiate (2 := fun (b : option sig) => match b with Some r3' => _ | None => _ end).
+                    destruct r3 as [ r3' | ].
+                    {
+                      eapply Move_Sem.
+                    }
+                    {
+                      eapply RealiseIn_monotone. eapply mono_Nop_Sem. omega. intros x y H. apply H.
+                    }
+                  }
+                }
+              }
+            }
+          }
+        }
+      }
+    - Unshelve. all: (cbn; omega).
+    - hnf. intros tin (yout&tout). intros H. hnf in H. destruct H as (r1&t1&(He&He')&H2); hnf in *; subst.
+      destruct (current _) eqn:E1; hnf in *.
+      {
+        destruct H2 as (->&->). split; auto. destruct (tout[@Fin.F1]); cbn in *; congruence.
+      }
+      {
+        destruct H2 as ((u1&t2)&H2&H3); hnf in *. destruct H2 as (->&H2); hnf in *; subst.
+        destruct H3 as (r1&H3); hnf in *. destruct H3 as (t3&(He&He')&H4); hnf in *; subst.
+        destruct (current (t3[@Fin.F1])) eqn:E2; hnf in *.
+        {
+          destruct H4 as (->&->). rewrite H2 in *. destruct (t1[@Fin.F1]); cbn in *; split; auto; congruence.
+        }
+        {
+          destruct H4 as ((u1&t2)&H4&H5); hnf in *. destruct H4 as (->&H4); hnf in *; subst.
+          destruct H5 as (r2&H5); hnf in *. destruct H5 as (t4&(He&He')&H5); hnf in *; subst.
+          destruct (current (t4[@Fin.F1])) eqn:E3; hnf in *.
+          {
+            destruct H5 as (->&H5). rewrite H2,H4,H5 in *. destruct (t1[@Fin.F1]); cbn in *; split; auto; congruence.
+          }
+          {
+            destruct H5 as (->&->). rewrite H2, H4 in *. destruct (t1[@Fin.F1]); cbn in *; split; auto; congruence.
+          }
+        }
+      }
+  Qed.
+
+End Peek.
